Refactor some definitions and add first lemmas (involuation).

src/dafny/ssz/Serialise.dfy
@@ -1,6 +1,7 @@
 
 include "../utils/NativeTypes.dfy"
 include "../utils/Eth2Types.dfy"
+include "../utils/Helpers.dfy"
 include "IntSeDes.dfy"
 include "BoolSeDes.dfy"
 
@@ -15,41 +16,67 @@ include "BoolSeDes.dfy"
     import opened Eth2Types
     import opened IntSeDes
     import opened BoolSeDes
-
-    /** The serialisable objects. */
-    datatype Serialisable = 
-            Uint8(n: uint8)
-        |   Bool(b: bool)
-
-    function method length(s: Serialisable) : nat {
-        match s
-        case Uint8(x) => 1
-        case Bool(b) => 1
-    }
+    import opened Helpers
 
     /** Encode/decode Uint8 yields Identity. */
     lemma uint8AsBytesInvolutive(n : uint8) 
         ensures bytesToUint8(uint8ToBytes(n)) == n
 
- 
-    function method serialise(s : Serialisable) : seq<Byte> 
+    /** Serialise.
+     *
+     *  @param  s   The object to serialise.
+     *  @returns    A sequence of bytes encoding `s`.
+     */
+    function serialise(s : Serialisable) : seq<Byte> 
     {
         match s 
-            case Bool(b) => boolToBytes(b)
+            case Bool(b, _) => boolToBytes(b)
 
-            case Uint8(n) => uint8ToBytes(n)
+            case Uint8(n, _) => uint8ToBytes(n)
     }
 
-    function method deserialise(xs : seq<Byte>, t : Serialisable) : Serialisable 
-        /* The lengths must match ... for now. */
-        requires length(t) == |xs|
+    /** Deserialise. 
+     *  
+     *  @param  xs  A sequence of bytes.
+     *  @param  s   A target type for the deserialised object.
+     *  @returns    Either a Success if `xs` could be deserialised
+     *              in an object of type s or a Failure oytherwise.
+     *  
+     *  @note       It would probabaly be good to return the suffix of `xs`
+     *              that has not been used in the deserialisation as well.
+     */
+    function deserialise(xs : seq<Byte>, s : Tipe) : Try<Serialisable>
     {
-        match t
-
-            case Bool(_) => Bool(bytesToBool(xs))
-
-            case Uint8(_) => Uint8(bytesToUint8(xs[0..1]))
+        match s
+            case Bool_ => if |xs| == 1 then
+                                Success(Bool(bytesToBool(xs), Bool_))
+                            else 
+                                Failure
+                            
+            case Uint8_ => if |xs| == 1 then
+                                Success(Uint8(bytesToUint8(xs[0..1]), Uint8_))
+                             else 
+                                Failure
     }
 
 
+    //  Specifications and Proofs
+    
+    /** 
+     * Well typed deserialisation does fail. 
+     */
+    lemma wellTypedDesNotFailure(s : Serialisable) 
+        requires wellTyped(s)
+        ensures deserialise(serialise(s), s.tipe) != Failure {
+            //  Thanks Dafny.
+        }
+    
+    /** 
+     * Deserialise(seriliase()) = Identity for well typed objects.
+     */
+    lemma seDesInvolutive(s : Serialisable, t: Tipe) 
+        requires wellTyped(s)
+        ensures deserialise(serialise(s), s.tipe) == Success(s) {
+            //  thanks Dafny.
+        }
  }
