src/dafny/utils/Helpers.dfy
@@ -1,0 +1,14 @@
+
+/** Helper types.  */
+module Helpers {
+
+    /** Try type (as in Scala). */
+    datatype Try<T> = Success(t : T) | Failure 
+
+    /* Option type */
+    datatype Option<T> = None | Some(T)
+
+    /* Either type */
+    datatype Either<T> = Left(T) | Right(T)
+
+}
